@prefix : <http://vocab.mmlab.org/vertere/terms#> .
@prefix owl: <http://www.w3.org/2002/07/owl#> .
@prefix rdf: <http://www.w3.org/1999/02/22-rdf-syntax-ns#> .
@prefix xml: <http://www.w3.org/XML/1998/namespace> .
@prefix xsd: <http://www.w3.org/2001/XMLSchema#> .
@prefix rdfs: <http://www.w3.org/2000/01/rdf-schema#> .
@prefix vertere: <http://vocab.mmlab.be/vertere/terms#> .
@base <http://vocab.mmlab.org/vertere/terms> .

<http://vocab.mmlab.org/vertere/terms> rdf:type owl:Ontology .


#################################################################
#
#    Object Properties
#
#################################################################


###  http://vocab.mmlab.org/vertere/terms#attribute

:attribute rdf:type owl:ObjectProperty ;
           
           rdfs:comment "Links an attribute to a resource (In Vertere, this is mostly fixed using a blank node)" .



###  http://vocab.mmlab.org/vertere/terms#identity

:identity rdf:type owl:ObjectProperty .



###  http://vocab.mmlab.org/vertere/terms#language

:language rdf:type owl:ObjectProperty ;
          
          rdfs:comment "The language of the attribute" ;
          
          rdfs:domain :Attribute .



###  http://vocab.mmlab.org/vertere/terms#lookup

:lookup rdf:type owl:ObjectProperty ;
        
        rdfs:range :Lookup ;
        
        rdfs:domain :Resource .



###  http://vocab.mmlab.org/vertere/terms#property

:property rdf:type owl:ObjectProperty ;
          rdfs:comment "The class of the property to map towards. This is for instance rdfs:label." ;
          
          rdfs:domain :Attribute ,
                      :Relationship .



###  http://vocab.mmlab.org/vertere/terms#relationship

:relationship rdf:type owl:ObjectProperty .



###  http://vocab.mmlab.org/vertere/terms#type

:type rdf:type owl:ObjectProperty ;
      
      rdfs:comment "Type that needs to be given to the resulting resource created" .





#################################################################
#
#    Data properties
#
#################################################################


###  http://vocab.mmlab.org/vertere/terms#base_uri

:base_uri rdf:type owl:DatatypeProperty ;
          
          rdfs:comment "A base URI is added to every relative URI used" .


:datatype rdf:type owl:DatatypeProperty ;
                 rdfs:comment "The data type of the object. This can be for instance an xsd:string" .

:value rdf:type owl:DatatypeProperty ;
               rdfs:comment "A fixed value which can be used to indicate an extra column. E.g. you can use this to add information about units used in another column." .

:source_column rdf:type owl:DatatypeProperty ;                      rdfs:comment "The source column key name to be used for this attribute" .

###  http://vocab.mmlab.org/vertere/terms#null_values

:null_values rdf:type owl:DatatypeProperty ;
             
             rdfs:comment "A list of strings that represent a NULL value in the datasource" .



###  http://vocab.mmlab.org/vertere/terms#type

:type rdf:type owl:DatatypeProperty ;
      
      rdfs:comment "Type that needs to be given to the resulting resource created" .





#################################################################
#
#    Classes
#
#################################################################


###  http://vocab.mmlab.org/vertere/terms#Attribute

:Attribute rdf:type owl:Class ;
           
           rdfs:comment "An attribute of a resource distilled from one or more source columns" .



###  http://vocab.mmlab.org/vertere/terms#Identity

:Identity rdf:type owl:Class .



###  http://vocab.mmlab.org/vertere/terms#Lookup

:Lookup rdf:type owl:Class .



###  http://vocab.mmlab.org/vertere/terms#Relationship

:Relationship rdf:type owl:Class .



###  http://vocab.mmlab.org/vertere/terms#Resource

:Resource rdf:type owl:Class ;
          
          rdfs:comment "A Vertere resource is a definition of a thing that can be identified using a source column value from the chunk of data given." .



###  http://vocab.mmlab.org/vertere/terms#Spec

:Spec rdf:type owl:Class ;
      
      rdfs:comment "A Vertere specification specifies how a chunk of data in an associative array structure can be mapped to RDF resources and attributes." .






###  Generated by the OWL API (version 3.4.2) http://owlapi.sourceforge.net

